Refactor RecordedNewViewMsgsContainSentVCMsgs.
RecordedNewViewMsgsContainSentVCMsgs changed to RecordedNewViewMsgsAreChecked.
In this new predicate we check whether the contents of each recorded new view msg
are correct according to the protocol (the VC msgs contained are valid and from different
senders, etc).
Temporary workaround in Library's MappedSetCardinality added to address Dafny's triggering problem.

docs/sbft-formal-model/proof.dfy
@@ -390,7 +390,7 @@ module Proof {
     && UnCommitableAgreesWithPrepare(c, v)
     && UnCommitableAgreesWithRecordedPrePrepare(c, v)//Unfinished proof.
     && HonestReplicasLeaveViewsBehind(c, v)
-    && RecordedNewViewMsgsContainSentVCMsgs(c, v)
+    && RecordedNewViewMsgsAreChecked(c, v)
     && RecordedViewChangeMsgsCameFromNetwork(c, v)
     && OneViewChangeMessageFromReplicaPerView(c, v)
     && SentViewChangesMsgsComportWithSentCommits(c, v)//Unfinished proof. This predicate is false.
@@ -1248,13 +1248,14 @@ module Proof {
     && (forall msg | msg in msgs :: c.clusterConfig.IsReplica(msg.sender))
   }
 
-  predicate {:opaque} RecordedNewViewMsgsContainSentVCMsgs(c:Constants, v:Variables) {
+  predicate {:opaque} RecordedNewViewMsgsAreChecked(c:Constants, v:Variables) {
     && v.WF(c)
     && (forall replicaIdx, newViewMsg | && IsHonestReplica(c, replicaIdx)
                                         && var replicaVariables := v.hosts[replicaIdx].replicaVariables;
                                         && newViewMsg in replicaVariables.newViewMsgsRecvd.msgs
                                            :: && newViewMsg.payload.vcMsgs.msgs <= v.network.sentMsgs
-                                              && MessagesAreFromReplicas(c, newViewMsg.payload.vcMsgs.msgs))
+                                              && MessagesAreFromReplicas(c, newViewMsg.payload.vcMsgs.msgs)
+                                              && newViewMsg.payload.checked(c.clusterConfig, v.network.sentMsgs))
   }
 
   predicate {:opaque} RecordedPrePreparesMatchHostView(c:Constants, v:Variables) {
@@ -1560,12 +1561,12 @@ module Proof {
     reveal_HonestReplicasLeaveViewsBehind();
   }
 
-  lemma HonestPreservesRecordedNewViewMsgsContainSentVCMsgs(c: Constants, v:Variables, v':Variables, step:Step, h_v:Replica.Variables, h_step:Replica.Step)
+  lemma HonestPreservesRecordedNewViewMsgsAreChecked(c: Constants, v:Variables, v':Variables, step:Step, h_v:Replica.Variables, h_step:Replica.Step)
     requires Inv(c, v)
     requires HonestReplicaStepTaken(c, v, v', step, h_v, h_step)
-    ensures RecordedNewViewMsgsContainSentVCMsgs(c, v')
+    ensures RecordedNewViewMsgsAreChecked(c, v')
   {
-    reveal_RecordedNewViewMsgsContainSentVCMsgs();
+    reveal_RecordedNewViewMsgsAreChecked();
     reveal_RecordedViewChangeMsgsCameFromNetwork();
 
     forall replicaIdx, newViewMsg | && IsHonestReplica(c, replicaIdx)
@@ -1645,9 +1646,12 @@ module Proof {
         var troubleMakers := ReplicasThatCanCommitInView(c, v', seqID, priorView, priorOperationWrapper);
         if |troubleMakers| >= c.clusterConfig.AgreementQuorum() {
           // Contradiction hypothesis
+          assert newViewMsg.payload.checked(c.clusterConfig, v.network.sentMsgs) by {
+            reveal_RecordedNewViewMsgsAreChecked();
+          }
           UniqueSendersCardinality(newViewMsg.payload.vcMsgs.msgs);
           assert viewChangers <= getAllReplicas(c) by {
-            reveal_RecordedNewViewMsgsContainSentVCMsgs();
+            reveal_RecordedNewViewMsgsAreChecked();
           }
           var doubleAgent := FindQuorumIntersection(c, viewChangers, troubleMakers);
           assert !c.clusterConfig.IsFaultyReplica(doubleAgent);
@@ -1656,7 +1660,7 @@ module Proof {
                                && vcMsg.sender == doubleAgent;
           assert vcMsg.payload.ViewChangeMsg?;
           assert vcMsg in v.network.sentMsgs by {
-            reveal_RecordedNewViewMsgsContainSentVCMsgs();
+            reveal_RecordedNewViewMsgsAreChecked();
           }
 
           assert !ReplicasInViewOrLower(c, v, seqID, priorView, priorOperationWrapper, doubleAgent) by {
@@ -1665,21 +1669,44 @@ module Proof {
           }
 
           if (seqID !in vcMsg.payload.certificates) {
-            assume false; // Need help from Oded in this branch.
+            reveal_TemporarilyDisableCheckpointing();
+            assume false;
+          } else if (vcMsg.payload.certificates[seqID].empty()) {
+            // Need help from Oded in this branch.
             // We are looking for an Inv that says every ViewChange msg after a Commit mentions the Committed SeqID.
+            assume false;
           } else {
-            var certView := vcMsg.payload.certificates[seqID].prototype().view; // We need to differentiate the first hop of the VC!!!
-            if certView <= priorView {
+            var certificate := vcMsg.payload.certificates[seqID];
+            var certView := certificate.prototype().view; // We need to differentiate the first hop of the VC!!!
+            if certView < priorView {
               assert !ReplicaSentCommit(c, v, seqID, priorView, priorOperationWrapper, doubleAgent) by {
                 // viewchangemessages from honest sender comport with uncommitable in view
                 //reveal_SentViewChangesMsgsComportWithUncommitableInView();
                 //assume false;
                 //reveal_CommitMsgsFromHonestSendersAgree();
                 reveal_EveryCommitMsgIsRememberedByVCMsgs();
-                assume EveryCommitMsgIsRememberedByVCMsgs(c, v);
+                assume EveryCommitMsgIsRememberedByVCMsgs(c, v);// TODO: put this predicate in the Inv.
               }
               assert doubleAgent !in troubleMakers;
               assert false;
+            } else if certView == priorView {
+              // Interesting branch - if there was a commit its operation wraper has to match the prepared certificate.
+              if ReplicaSentCommit(c, v, seqID, priorView, priorOperationWrapper, doubleAgent) {
+                // operation wrapers agree
+                var sentCommit := Network.Message(doubleAgent,
+                                                  Messages.Commit(priorView,
+                                                                  seqID,
+                                                                  priorOperationWrapper));
+                assert sentCommit in v.network.sentMsgs;
+                assert CertificateComportsWithCommit(c, certificate, sentCommit) by {
+                  reveal_EveryCommitMsgIsRememberedByVCMsgs();
+                  assume EveryCommitMsgIsRememberedByVCMsgs(c, v);// TODO: put this predicate in the Inv.
+                }
+                assert sentCommit.payload.operationWrapper == certificate.prototype().operationWrapper;
+              } else {
+                assert doubleAgent !in troubleMakers;
+                assert false;
+              }
             } else { // certView > priorView // Use the mutual induction hypothesis to get UncommitableInView directly.
               /*
                 Grab the cert
@@ -2158,7 +2185,7 @@ module Proof {
       HonestPreservesUnCommitableAgreesWithRecordedPrePrepare(c, v, v', step, h_v, h_step);
       HonestPreservesUnCommitableAgreesWithPrepare(c, v, v', step, h_v, h_step);
       HonestPreservesHonestReplicasLeaveViewsBehind(c, v, v', step, h_v, h_step);
-      HonestPreservesRecordedNewViewMsgsContainSentVCMsgs(c, v, v', step, h_v, h_step);
+      HonestPreservesRecordedNewViewMsgsAreChecked(c, v, v', step, h_v, h_step);
       HonestPreservesRecordedViewChangeMsgsCameFromNetwork(c, v, v', step, h_v, h_step);
       HonestPreservesSentViewChangesMsgsComportWithSentCommits(c, v, v', step, h_v, h_step);
       HonestPreservesEveryCommitMsgIsRememberedByItsSender(c, v, v', step, h_v, h_step);
@@ -2244,8 +2271,8 @@ module Proof {
     assert HonestReplicasLeaveViewsBehind(c, v') by {
       reveal_HonestReplicasLeaveViewsBehind();
     }
-    assert RecordedNewViewMsgsContainSentVCMsgs(c, v') by {
-      reveal_RecordedNewViewMsgsContainSentVCMsgs();
+    assert RecordedNewViewMsgsAreChecked(c, v') by {
+      reveal_RecordedNewViewMsgsAreChecked();
     }
     assert RecordedViewChangeMsgsCameFromNetwork(c, v') by {
       reveal_RecordedViewChangeMsgsCameFromNetwork();
@@ -2294,7 +2321,7 @@ module Proof {
       reveal_UnCommitableAgreesWithPrepare();
       reveal_UnCommitableAgreesWithRecordedPrePrepare();
       reveal_HonestReplicasLeaveViewsBehind();
-      reveal_RecordedNewViewMsgsContainSentVCMsgs();
+      reveal_RecordedNewViewMsgsAreChecked();
       reveal_RecordedViewChangeMsgsCameFromNetwork();
       reveal_SentViewChangesMsgsComportWithSentCommits();
       reveal_EveryCommitMsgIsRememberedByItsSender();
